code/ecdsap256/Hacl.Impl.P256.Q.PrimitivesMasking.fst
@@ -14,6 +14,7 @@ open Spec.P256.Lemmas
 
 #set-options "--z3rlimit 300" 
 
+[@CInline]
 val cmovznz4: out: felem -> x: felem -> y: felem -> mask: uint64 -> Stack unit
   (requires fun h -> live h out /\ live h x /\ live h y /\ (uint_v mask == 0 \/ uint_v mask = pow2 64 - 1))
   (ensures fun h0 _ h1 -> modifies (loc out) h0 h1 /\ (
@@ -47,7 +48,7 @@ let cmovznz4 out x y mask =
   cmovznz4_lemma mask (Seq.index y 3) (Seq.index x 3)
 
 
-
+[@CInline]
 val copy_conditional: out: felem -> x: felem -> mask: uint64{uint_v mask = 0 \/ uint_v mask = pow2 64 - 1} -> Stack unit 
   (requires fun h -> live h out /\ live h x)
   (ensures fun h0 _ h1 -> modifies (loc out) h0 h1 /\ 
